check for disjointness; copy input buffer to avoid double fetches

steel/Zeta.Steel.ExternalPtr.fst
@@ -1,14 +1,52 @@
 module Zeta.Steel.ExternalPtr
+open Steel.ST.GenElim
 
-let extern_ptr = A.array U8.t
+let extern_input_ptr = A.array U8.t
 
-let gtake p = p
+[@@__reduce__]
+let has_extern_input_ptr0 e n =
+  exists_ (fun p -> exists_ (fun contents -> A.pts_to e p contents)) `star`
+  pure (U32.v n == A.length e)
+
+let has_extern_input_ptr e n =
+  has_extern_input_ptr0 e n
 
 assume
 val enclave_api_validate (x:A.array U8.t) (n: U32.t) : Pure bool
   (requires True)
   (ensures (fun b -> b == true ==> U32.v n == A.length x))
 
-let valid = enclave_api_validate
+let valid_input = enclave_api_validate
+
+let copy_extern_input_ptr
+  e n
+=
+  let res = A.alloc 0uy n in
+  rewrite (has_extern_input_ptr e n) (has_extern_input_ptr0 e n);
+  let _ = gen_elim () in
+  A.memcpy e res n;
+  rewrite (has_extern_input_ptr0 e n) (has_extern_input_ptr e n);
+  return res
+
+let extern_output_ptr = A.array U8.t
+
+let gtake p = p
+
+let valid_output = enclave_api_validate
 
 let take x n = x
+
+assume
+val enclave_api_check_input_output_disjoint
+  (input: extern_input_ptr)
+  (input_len: U32.t)
+  (output: extern_output_ptr)
+  (output_len: U32.t)
+  (output_contents: Ghost.erased (Seq.seq U8.t))
+: ST bool
+    (has_extern_input_ptr input input_len `sl_and` A.pts_to (gtake output) full_perm output_contents)
+    (fun b -> check_disjoint_post b (has_extern_input_ptr input input_len) (A.pts_to (gtake output) full_perm output_contents))
+    (valid_input input input_len /\ valid_output output output_len)
+    (fun _ -> True)
+
+let check_input_output_disjoint = enclave_api_check_input_output_disjoint
