steel/Zeta.Steel.ExternalPtr.fsti
@@ -1,4 +1,5 @@
 module Zeta.Steel.ExternalPtr
+include Zeta.Steel.ExternalPtr.SLAnd
 
 // DO NOT FRIEND this module!
 
@@ -6,17 +7,56 @@ module A = Steel.ST.Array
 module U32 = FStar.UInt32
 module U8 = FStar.UInt8
 
-inline_for_extraction
-val extern_ptr : Type0
-
-val gtake (p: extern_ptr) : GTot (A.array U8.t)
+open Steel.ST.Util
 
 inline_for_extraction
-val valid (p: extern_ptr) (n: U32.t) : Pure bool
+val extern_input_ptr : Type0
+
+val has_extern_input_ptr (e: extern_input_ptr) (n: U32.t) : vprop
+
+inline_for_extraction
+val valid_input (p: extern_input_ptr) (n: U32.t) : Tot bool
+
+inline_for_extraction
+val copy_extern_input_ptr
+  (e: extern_input_ptr)
+  (n: U32.t)
+: ST (A.array U8.t)
+    (has_extern_input_ptr e n)
+    (fun res -> has_extern_input_ptr e n `star` exists_ (fun contents -> A.pts_to res full_perm contents))
+    (valid_input e n)
+    (fun res -> A.is_full_array res /\ A.length res == U32.v n)
+
+inline_for_extraction
+val extern_output_ptr: Type0
+
+val gtake (p: extern_output_ptr) : GTot (A.array U8.t)
+
+inline_for_extraction
+val valid_output (p: extern_output_ptr) (n: U32.t) : Pure bool
   (requires True)
   (ensures (fun b -> b == true ==> U32.v n == A.length (gtake p)))
 
 inline_for_extraction
-val take (p: extern_ptr) (n: Ghost.erased U32.t) : Pure (A.array U8.t)
-  (requires (valid p n))
+val take (p: extern_output_ptr) (n: Ghost.erased U32.t) : Pure (A.array U8.t)
+  (requires (valid_output p n))
   (ensures (fun y -> y == gtake p))
+
+let check_disjoint_post
+  (b: bool)
+  (p1 p2: vprop)
+: vprop
+= p1 `(if b then star else sl_and)` p2
+
+inline_for_extraction
+val check_input_output_disjoint
+  (input: extern_input_ptr)
+  (input_len: U32.t)
+  (output: extern_output_ptr)
+  (output_len: U32.t)
+  (output_contents: Ghost.erased (Seq.seq U8.t))
+: ST bool
+    (has_extern_input_ptr input input_len `sl_and` A.pts_to (gtake output) full_perm output_contents)
+    (fun b -> check_disjoint_post b (has_extern_input_ptr input input_len) (A.pts_to (gtake output) full_perm output_contents))
+    (valid_input input input_len /\ valid_output output output_len)
+    (fun _ -> True)
