steel/Zeta.Steel.ExternalPtr.SLAnd.fst
@@ -1,0 +1,20 @@
+module Zeta.Steel.ExternalPtr.SLAnd
+friend Steel.Memory
+friend Steel.Heap
+
+module SEA = Steel.Effect.Atomic
+module SC = Steel.ST.Coercions
+
+let sl_and p1 p2 =
+  to_vprop (hp_of p1 `Steel.Memory.h_and` hp_of p2)
+
+let star_sl_and' (#opened: _) (p1 p2: vprop) : SEA.SteelGhostT unit opened
+  (p1 `star` p2)
+  (fun _ -> p1 `sl_and` p2)
+= SEA.rewrite_slprop
+    (p1 `star` p2)
+    (p1 `sl_and` p2)
+    (fun m -> () (* works thanks to `friend`ing *) )
+
+let star_sl_and p1 p2 =
+  SC.coerce_ghost (fun _ -> star_sl_and' p1 p2)
